atomic_pair.v
@@ -1,0 +1,96 @@
+From iris.program_logic Require Export weakestpre hoare.
+From iris.proofmode Require Import invariants ghost_ownership.
+From iris.heap_lang Require Export lang.
+From iris.heap_lang Require Import proofmode notation.
+From iris.heap_lang.lib Require Import spin_lock.
+From iris.tests Require Import atomic.
+From iris.algebra Require Import dec_agree frac.
+From iris.program_logic Require Import auth.
+From flatcomb Require Import sync.
+Import uPred.
+
+Section atomic_pair.
+  Context `{!heapG Σ, !lockG Σ, !syncG Σ} (N : namespace).
+  
+  Definition pcas_seq : val :=
+    λ: "ls" "ab",
+       if: !(Fst "ls") = Fst "ab"
+         then if: !(Snd "ls") = Fst "ab"
+                then Fst "ls" <- Snd "ab";; Snd "ls" <- Snd "ab";; #true
+                else #false
+         else #false.
+
+  Local Opaque pcas_seq.
+
+  Definition α (x: val) : iProp Σ := (∃ a b: val, x = (a, b)%V)%I.
+  
+  Definition ϕ (ls: val) (xs: val) : iProp Σ :=
+    (∃ (l1 l2: loc) (x1 x2: val),
+       ls = (#l1, #l2)%V ★ xs = (x1, x2)%V ★ l1 ↦ x1 ★ l2 ↦ x2)%I.
+
+  Definition β (ab: val) (xs xs': val) (v: val) : iProp Σ :=
+    (■ ∃ a b x1 x2 x1' x2': val,
+         ab = (a, b)%V ∧ xs = (x1, x2)%V ∧ xs' = (x1', x2')%V ∧
+         ((v = #true  ∧ x1 = a ∧ x2 = a ∧ x1' = b ∧ x2' = b) ∨
+          (v = #false ∧ (x1 ≠ a ∨ x2 ≠ a) ∧ xs = xs')))%I.
+
+  Local Opaque β.
+  
+  Lemma pcas_seq_spec: seq_spec N pcas_seq ϕ α β ⊤.
+  Proof.
+    rewrite /seq_spec.
+    intros Φ l.
+    iIntros "!# _". wp_seq. iVsIntro. iPureIntro. clear Φ.
+    iIntros (x Φ g HN) "(#Hh & Hg & Hα & HΦ)".
+    rewrite /ϕ /α.
+    iDestruct "Hg" as (l1 l2 x1 x2) "(% & % & Hl1 & Hl2)".
+    iDestruct "Hα" as (a b) "%".
+    subst. simpl. wp_let. wp_proj. wp_load. wp_proj.
+    wp_op=>[?|Hx1na].
+    - subst.
+      wp_if. wp_proj. wp_load. wp_proj.
+      wp_op=>[?|Hx2na]. subst.
+      + wp_if. wp_proj. wp_proj. wp_store. wp_proj. wp_proj. wp_store.
+        iDestruct ("HΦ" $! #true (b, b)%V) as "HΦ".
+        iApply ("HΦ" with "[Hl1 Hl2]").
+        { iExists l1, l2, b, b. iFrame. eauto. }
+        rewrite /β.
+        iPureIntro. exists a, b, a, a, b, b. repeat (split; first done). left. eauto.
+      + wp_if.
+        iDestruct ("HΦ" $! #false (a, x2)%V) as "H".
+        iApply ("H" with "[Hl1 Hl2]").
+        { iExists l1, l2, a, x2. iFrame. eauto. }
+        rewrite /β.
+        iPureIntro. exists a, b, a, x2, a, x2. repeat (split; first done). right. eauto.
+    - subst.
+      wp_if.
+      iDestruct ("HΦ" $! #false (x1, x2)%V) as "H".
+      iApply ("H" with "[Hl1 Hl2]").
+      { iExists l1, l2, x1, x2. iFrame. eauto. }
+      rewrite /β.
+      iPureIntro. exists a, b, x1, x2, x1, x2. repeat (split; first done). right. eauto.
+  Qed.
+
+  Lemma pcas_atomic_spec:
+    heapN ⊥ N → heap_ctx ⊢ WP sync (λ: <>, (ref #0, ref #0))%V pcas_seq {{ f, ∃ γ, gFrag γ (#0, #0) ★ ∀ x, □ atomic_triple' α β ⊤ ⊤ f x γ  }}.
+  Proof.
+    iIntros (HN) "#Hh".
+    iDestruct (atomic_spec with "[]") as "Hspec"=>//.
+    - apply pcas_seq_spec.
+    - rewrite /cons_spec.
+      iIntros (Φ _) "[#Hh HΦ]".
+      wp_seq.
+      wp_alloc l1 as "Hl1".
+      wp_alloc l2 as "Hl2".
+      iVs (own_alloc (gFullR (#0, #0) ⋅ gFragR (#0, #0))) as (γ) "[HgFull HgFrag]"; first by done.
+      rewrite /ϕ.
+      iSpecialize ("HΦ" $! (#l1, #l2)%V γ).
+      rewrite /gFull /gFrag.
+      iVsIntro.
+      iAssert ((∃ (l0 l3 : loc) (x1 x2 : val),
+            (#l1, #l2)%V = (#l0, #l3)%V
+            ★ (#0, #0)%V = (x1, x2)%V ★ l0 ↦ x1 ★ l3 ↦ x2))%I with "[Hl1 Hl2]" as "H'".
+      { iExists l1, l2, #0, #0. iFrame. eauto. }
+      iApply ("HΦ" with "H' HgFull HgFrag").
+   Qed.
+End atomic_pair.
